@prefix owl: <http://www.w3.org/2002/07/owl#> .
@prefix dc: <http://purl.org/dc/terms/> .
@prefix ns0: <http://purl.org/vocab/vann/> .
@prefix rdfs: <http://www.w3.org/2000/01/rdf-schema#> .
@prefix foaf: <http://xmlns.com/foaf/0.1/> .
@prefix cc: <http://creativecommons.org/ns#> .
@prefix xsd: <http://www.w3.org/2001/XMLSchema#> .
@prefix skos: <http://www.w3.org/2004/02/skos/core#> .
@prefix schema: <http://schema.org/> .
@prefix bont: <http://ontology.bonsai.uno/core#> .
@prefix om2: <http://www.ontology-of-units-of-measure.org/resource/om-2/> .
@prefix time: <http://www.w3.org/2006/time#> .

##############################################

# Metadata

##############################################



<http://ontology.bonsai.uno/core>
  a owl:Ontology ;
  dc:title "The BONSAI ontology"@en ;
  dc:description "The BONSAI ontologies provides elements of description for product footprint concepts defined in the bonsai.uno data base"@en ;
  foaf:homepage <http://ontology.bonsai.uno/core/documentation.html> ;
  ns0:preferredNamespacePrefix "bont" ;
  ns0:preferredNamespaceUri "http://ontology.bonsai.uno/core#" ;
  rdfs:isDefinedBy <http://ontology.bonsai.uno/core/ontology_v0.2.rdf> ;
  owl:versionInfo "Version 0.2 - 2022-03-15"@en ;
  dc:modified "2022-03-15"^^xsd:date ;
  dc:publisher "bonsai.uno" ;
  dc:creator <http://bonsai.uno/foaf/bonsai.rdf#bonsai> ;
  dc:contributor "Matteo Lissandrini", "Agneta Ghose", "Bo Weidemma" ;
  cc:license <http://creativecommons.org/licenses/by/3.0/> ;
  rdfs:comment """Bonsai ontology version 0.2 :
                based on changes discussed on Jan2020!
               """@en .



##############################################

# Classes definitions

##############################################


<http://ontology.bonsai.uno/core#Activity>
  a owl:Class ;
  rdfs:comment "Activity is the act of making or doing something which is defined both spatially and temporally. This is one of the identifying dimensions of a datapoint. This class defines multiple properties on the type and direction of flows. ‘Process’ is a commonly used synonym in other LCA databases."@en ;
  rdfs:label "Activity"@en ;
  rdfs:subClassOf skos:ConceptScheme .


<http://ontology.bonsai.uno/core#ActivityType>
  a owl:Class ;
  rdfs:comment "The type of an activity, e.g, stock accumulation, steel production, etc. This class includes the labels of activities. Includes both human activities and environmental mechanisms."@en ;
  rdfs:label "Activity Type"@en ;
  rdfs:subClassOf skos:ConceptScheme .


<http://ontology.bonsai.uno/core#Flow>
  a owl:Class ;
  rdfs:comment " An input or output of an entity to or from an instance of an Activity or a directional exchange of an entity between two instances of Activity. This class contains the quantity of the entity (Flow Object) that is consumed as input or produced as output of an Activity."@en ;
  rdfs:label "Flow"@en ;
  rdfs:subClassOf skos:ConceptScheme, om2:Measure .


<http://ontology.bonsai.uno/core#FlowObject>
  a owl:Class ;
  rdfs:comment "This class includes the labels of entities that are produced or consumed by an activity or added to or removed from a stock accumulation."@en ;
  rdfs:label "Flow Object"@en ;
  rdfs:subClassOf skos:ConceptScheme .


<http://ontology.bonsai.uno/core#BalanceableProperty>
  a owl:Class ;
  rdfs:comment "A quantity for which the sum for all input flows must equal the sum for all output flows. A quantity that follows a conservation law. Balanceable properties are particularly relevant for validating the completeness and consistency of an Activity description or a database of such activities. "@en ;
  rdfs:label "Balanceable Property"@en ;
  rdfs:subClassOf skos:ConceptScheme, om2:Measure .


<http://ontology.bonsai.uno/core#BalanceablePropertyType>
  a owl:Class ;
  rdfs:comment "Contains the labels of BalanceableProperty such as dry mass, wet mass, elemental mass, person-time, monetary value."@en ;
  rdfs:label "Balanceable Property Type"@en ;
  rdfs:subClassOf skos:ConceptScheme, om2:Quantity .


<http://ontology.bonsai.uno/core#Agent>
  a owl:Class ;
  rdfs:comment "An entity (person or thing) that performs an activity, usually it has a specific location."@en ;
  rdfs:label "Agent"@en ;
  rdfs:subClassOf skos:ConceptScheme .



<http://ontology.bonsai.uno/core#ReferenceUnit>
  a owl:Class ;
  rdfs:comment " The measure to which the numeric value representing the measure of a Flow is expressed 'in proportion to'. In LCA, the term ‘Functional Unit’ is defined as a common ReferenceUnit for all activities in an LCA study."@en ;
  rdfs:label "Reference Unit"@en ;
  rdfs:subClassOf skos:ConceptScheme, om2:Measure .




xsd:integer a rdfs:Datatype .
xsd:float a rdfs:Datatype .




##############################################

# Property definitions

##############################################


<http://ontology.bonsai.uno/core#isInputOf>
  a owl:FunctionalProperty, owl:ObjectProperty ;
  rdfs:comment "Specifies the Activity that a Flow is an input to."@en ;
  rdfs:domain bont:Flow ;
  rdfs:label "input of"@en ;
  rdfs:range bont:Activity .


<http://ontology.bonsai.uno/core#isOutputOf>
  a owl:FunctionalProperty, owl:ObjectProperty ;
  rdfs:comment "Specifies the Activity that a Flow is an output of."@en ;
  rdfs:domain bont:Flow ;
  rdfs:label "output of"@en ;
  rdfs:range bont:Activity .

<http://ontology.bonsai.uno/core#hasObjectType>
  a owl:FunctionalProperty, owl:ObjectProperty ;
  rdfs:comment "Specifies the Flow object consumed or produced."@en ;
  rdfs:domain bont:Flow ;
  rdfs:label "object type"@en ;
  rdfs:range bont:FlowObject ;
  rdfs:subPropertyOf dc:type .


<http://ontology.bonsai.uno/core#hasDeterminingFlow>
  a owl:FunctionalProperty, owl:ObjectProperty ;
  rdfs:comment "Specifies a specific flow object produced or consumed by an activity for which a change in demand or supply will affect the activity level (such as its production volume or extent)."@en ;
  rdfs:domain bont:Activity ;
  rdfs:label "determining flow"@en ;
  rdfs:range bont:Flow .



<http://ontology.bonsai.uno/core#hasActivityType>
  a owl:ObjectProperty ;
  rdfs:comment "Specifies the label of an Activity."@en ;
  rdfs:domain bont:Activity ;
  rdfs:label "activity type"@en ;
  rdfs:range bont:ActivityType ;
  rdfs:subPropertyOf dc:type .


<http://ontology.bonsai.uno/core#performs>
  a owl:ObjectProperty ;
  rdfs:comment "Specifies the Agent who performs an activity."@en ;
  rdfs:domain bont:Agent ;
  rdfs:label "performs"@en ;
  rdfs:range bont:Activity .



<http://ontology.bonsai.uno/core#hasTemporalExtent>
  a owl:FunctionalProperty, owl:ObjectProperty ;
  rdfs:comment "Specifies the temporal extent for an activity."@en ;
  rdfs:domain bont:Activity ;
  rdfs:label "temporal extent"@en ;
  rdfs:range time:ProperInterval .


<http://ontology.bonsai.uno/core#hasLocation>
  a owl:FunctionalProperty, owl:ObjectProperty ;
  rdfs:comment "Specifies the location of an Activity or Agent"@en ;
  rdfs:domain [ rdfs:type owl:Class ;
                   owl:unionOf ( bont:Activity
                                 bont:Agent
                   ) ];
  rdfs:label "located at"@en ;
  rdfs:range schema:location .



<http://ontology.bonsai.uno/core#isProportionalTo>
  a owl:FunctionalProperty, owl:ObjectProperty ;
  rdfs:comment "Specifies the reference unit that the amount of a BalanceableProperty of a Flow is proportional to."@en ;
  rdfs:domain bont:BalanceableProperty ;
  rdfs:label "proportional to"@en ;
  rdfs:range bont:ReferenceUnit .

<http://ontology.bonsai.uno/core#hasBalanceableProperty>
  a owl:FunctionalProperty, owl:ObjectProperty ;
  rdfs:comment "Specifies the  Measure of a Flow when this Measure is a BalanceableProperty, i.e. when it follows a conservation law."@en ;
  rdfs:domain bont:Flow ;
  rdfs:label "has balanceable property"@en ;
  rdfs:range bont:BalanceableProperty . 

<http://ontology.bonsai.uno/core#hasPropertyType>
  a owl:FunctionalProperty, owl:ObjectProperty ;
  rdfs:comment "Specifies the dimension (Quantity) of a Measure that is classified as a BalanceableProperty."@en ;
  rdfs:domain bont:BalanceableProperty ;
  rdfs:label "property type"@en ;
  rdfs:range bont:BalanceablePropertyType .


<http://ontology.bonsai.uno/core#hasReferenceFlowObject>
  a owl:FunctionalProperty, owl:ObjectProperty ;
  rdfs:comment "Specifies a FlowObject that functions as the ReferenceUnit for a BalanceableProperty measure."@en ;
  rdfs:domain bont:ReferenceUnit ;
  rdfs:label "references flow object"@en ;
  rdfs:range bont:FlowObject .

